checkpoint specifying a file system in the trace infrastructure
mostly failed, it seems, because separation logic doesn't work well
with commuting

src/FS/FSAPI.v
@@ -7,23 +7,6 @@ Require Import FS.SepLogic.Mem.
 Require Import FS.SepLogic.Pred.
 
 
-Definition pointed_set (T : Type) : Type := T * list T.
-
-Definition set_add {T} (s : pointed_set T) (v : T) := (v, fst s :: snd s).
-
-Definition set_latest {T} (s : pointed_set T) := fst s.
-
-Definition set_older {T} (s : pointed_set T) := snd s.
-
-Definition set_transform {T} (s s' : pointed_set T) (rel : T -> T -> Prop) :=
-  rel (fst s) (fst s') /\
-  Forall2 rel (snd s) (snd s').
-
-Definition set_in {T} (v : T) (s : pointed_set T) :=
-  v = fst s \/
-  In v (snd s).
-
-
 Record file := mk_file {
   FileData : string;
 }.
@@ -39,7 +22,7 @@ Inductive tree_node :=
 Definition pathname := list string.
 
 
-Definition State := pointed_set (mem pathname tree_node).
+Definition State := mem pathname tree_node.
 
 (* One interesting difference from FSCQ's DirSep: the memory contains
   [Some Missing] entries for files that do not exist in an existing directory,
@@ -80,6 +63,7 @@ Global Opaque maildir.
 Global Opaque tmpdir.
 
 
+(*
 Axiom fs_concur : forall (tid : string) (p : pred pathname tree_node), pred pathname tree_node.
 Axiom fs_concur_star : forall tid p1 p2,
   fs_concur tid (p1 * p2) ===> fs_concur tid p1 * fs_concur tid p2.
@@ -109,6 +93,7 @@ Admitted.
 Lemma fs_concur_exists : forall tid T (p : T -> _),
   fs_concur tid (exists x, p x) ===> exists x, fs_concur tid (p x).
 Admitted.
+*)
 
 Lemma subtree_pred_exists : forall pn T (p : T -> _),
   subtree_pred pn (exists x, p x) ===> exists x, subtree_pred pn (p x).
@@ -124,215 +109,257 @@ Admitted.
 
 
 Definition inited (s : State) : Prop :=
-  set_older s = nil /\
-  set_latest s |= nil |-> Dir 0 * empty_dir.
+  s |= nil |-> Dir 0 * empty_dir.
 
-Definition create_spec tid dir name : Specification _ _ unit State :=
-  fun '(F, dirnum) state => {|
-    pre :=
-      set_latest state |= F * dir |-> Dir dirnum * (dir ++ [name]) |-> Missing;
-    post := fun r state' =>
-      exists handle m,
-      r = handle /\
-      m |= fs_concur tid (F * dir |-> Dir dirnum * (dir ++ [name]) |-> File handle empty_file) /\
-      (forall mold,
-       set_in mold state ->
-       ~ exists F' pn f', mold |= F' * pn |-> File handle f') /\
-      state' = set_add state m;
-    recovered := fun _ _ => False
-  |}.
 
-Definition mkdir_spec tid dir name : Specification _ _ unit State :=
-  fun '(F, dirnum) state => {|
-    pre :=
-      set_latest state |= F * dir |-> Dir dirnum * (dir ++ [name]) |-> Missing;
-    post := fun r state' =>
-      exists newdirnum m,
-      r = newdirnum /\
-      m |= fs_concur tid (F * dir |-> Dir dirnum * (dir ++ [name]) |-> Dir newdirnum *
-           subtree_pred (dir ++ [name]) empty_dir) /\
-      state' = set_add state m;
-    recovered := fun _ _ => False
-  |}.
-
-Definition delete_spec tid pn : Specification _ _ unit State :=
-  fun '(F, handle, f) state => {|
-    pre :=
-      set_latest state |= F * pn |-> File handle f;
-    post := fun r state' =>
-      exists m,
-      r = tt /\
-      m |= fs_concur tid (F * pn |-> Missing) /\
-      state' = set_add state m;
-    recovered := fun _ _ => False
-  |}.
-
-Definition rmdir_spec tid pn : Specification _ _ unit State :=
-  fun '(F, dirnum) state => {|
-    pre :=
-      set_latest state |= F * pn |-> Dir dirnum * subtree_pred pn empty_dir;
-    post := fun r state' =>
-      exists m,
-      r = tt /\
-      m |= fs_concur tid (F * pn |-> Missing) /\
-      state' = set_add state m;
-    recovered := fun _ _ => False
-  |}.
 
 Inductive stat_result :=
 | StatMissing
 | StatFile
 | StatDir.
 
-Definition stat_spec dirpn name : Specification _ _ unit State :=
-  fun '(F, dirnum) state => {|
-    pre :=
-      set_latest state |= F * dirpn |-> Dir dirnum;
-    post := fun r state' =>
-      state' = state /\
-      ((r = StatFile /\ exists F' handle f,
-        F' * (dirpn ++ [name]) |-> File handle f ===> F) \/
-       (r = StatDir /\ exists F' dirinum,
-        F' * (dirpn ++ [name]) |-> Dir dirinum ===> F) \/
-       (r = StatMissing /\ exists F',
-        F' * (dirpn ++ [name]) |-> Missing ===> F));
-    recovered := fun _ _ => False
-  |}.
-
-Definition readdir_spec dirpn : Specification _ _ unit State :=
-  fun '(F, dirnum) state => {|
-    pre :=
-      set_latest state |= F * dirpn |-> Dir dirnum;
-    post := fun r state' =>
-      state' = state /\
-      forall fn,
-      ((In fn r /\ exists F' handle f,
-        F' * (dirpn ++ [fn]) |-> File handle f ===> F) \/
-       (In fn r /\ exists F' dirinum,
-        F' * (dirpn ++ [fn]) |-> Dir dirinum ===> F) \/
-       (~ In fn r /\ exists F',
-        F' * (dirpn ++ [fn]) |-> Missing ===> F));
-    recovered := fun _ _ => False
-  |}.
-
-Definition rename_file_spec pn dstdir dstname : Specification _ _ unit State :=
-  fun '(F, handle, f, dirnum) state => {|
-    pre :=
-      set_latest state |= F * pn |-> File handle f *
-               dstdir |-> Dir dirnum * (dstdir ++ [dstname]) |-> Missing;
-    post := fun r state' =>
-      exists m,
-      r = tt /\
-      m |= F * pn |-> Missing *
-           dstdir |-> Dir dirnum * (dstdir ++ [dstname]) |-> File handle f /\
-      state' = set_add state m;
-    recovered := fun _ _ => False
-  |}.
-
-Definition read_spec pn : Specification _ _ unit State :=
-  fun '(F, handle, f) state => {|
-    pre :=
-      set_latest state |= F * pn |-> File handle f;
-    post := fun r state' =>
-      r = FileData f /\
-      state' = state;
-    recovered := fun _ _ => False
-  |}.
-
-Definition write_logged_spec pn data : Specification _ _ unit State :=
-  fun '(F, handle, f0) state => {|
-    pre :=
-      set_latest state |= F * pn |-> File handle f0;
-    post := fun r state' =>
-      exists m,
-      r = tt /\
-      m |= F * pn |-> File handle (mk_file data) /\
-      state' = set_add state m;
-    recovered := fun _ _ => False
-  |}.
-
-Definition write_bypass_relation (handle : nat) (f : file) (m m' : mem pathname tree_node) : Prop :=
-  (forall F pn f0, m |= F * pn |-> File handle f0 -> m' |= F * pn |-> File handle f) /\
-  ((~ exists F pn f0, m |= F * pn |-> File handle f0) -> m' = m).
-
-Definition write_bypass_spec pn data : Specification _ _ unit State :=
-  fun '(F, filenum, f0) state => {|
-    pre :=
-      set_latest state |= F * pn |-> File filenum f0;
-    post := fun r state' =>
-      r = tt /\
-      set_transform state state' (write_bypass_relation filenum (mk_file data));
-    recovered := fun _ _ => False
-  |}.
-
-Definition find_available_name_spec tid dirpn : Specification _ _ unit State :=
-  fun '(F, dirnum) state => {|
-    pre :=
-      set_latest state |= F * dirpn |-> Dir dirnum;
-    post := fun r state' =>
-      exists suffix, r = (tid ++ "."%string ++ suffix)%string /\
-      state' = state /\
-      set_latest state |= fs_concur tid (pred_eexcept F (dirpn ++ [r]) * (dirpn ++ [r]) |-> Missing * dirpn |-> Dir dirnum);
-    recovered := fun _ _ => False
-  |}.
-
-Definition debug_spec : Specification _ _ unit State :=
-  fun (_: unit) state => {|
-    pre := True;
-    post := fun r state' => state = state' /\ r = tt;
-    recovered := fun _ _ => False
-  |}.
-
-Module Type FSAPI.
-
-  Axiom init : proc InitResult.
-  Axiom create : pathname -> string -> proc nat.
-  Axiom mkdir : pathname -> string -> proc nat.
-  Axiom delete : pathname -> proc unit.
-  Axiom rmdir : pathname -> proc unit.
-  Axiom rename_file : pathname -> pathname -> string -> proc unit.
-  Axiom read : pathname -> proc string.
-  Axiom write_logged : pathname -> string -> proc unit.
-  Axiom write_bypass : pathname -> string -> proc unit.
-  Axiom stat : pathname -> string -> proc stat_result.
-  Axiom readdir : pathname -> proc (list string).
-  Axiom recover : proc unit.
-  Axiom find_available_name : pathname -> proc string.
-  Axiom debug: string -> proc unit.
-  
-  Axiom abstr : Abstraction State.
-
-  Axiom init_ok : init_abstraction init recover abstr inited.
-  Axiom create_ok : forall tid dir name, proc_spec (create_spec tid dir name) (create dir name) recover abstr.
-  Axiom mkdir_ok : forall tid dir name, proc_spec (mkdir_spec tid dir name) (mkdir dir name) recover abstr.
-  Axiom delete_ok : forall tid pn, proc_spec (delete_spec tid pn) (delete pn) recover abstr.
-  Axiom rmdir_ok : forall tid pn, proc_spec (rmdir_spec tid pn) (rmdir pn) recover abstr.
-  Axiom rename_file_ok : forall pn newdir newname, proc_spec (rename_file_spec pn newdir newname) (rename_file pn newdir newname) recover abstr.
-  Axiom read_ok : forall pn, proc_spec (read_spec pn) (read pn) recover abstr.
-  Axiom write_logged_ok : forall pn f, proc_spec (write_logged_spec pn f) (write_logged pn f) recover abstr.
-  Axiom write_bypass_ok : forall pn f, proc_spec (write_bypass_spec pn f) (write_bypass pn f) recover abstr.
-  Axiom stat_ok : forall pn n, proc_spec (stat_spec pn n) (stat pn n) recover abstr.
-  Axiom readdir_ok : forall pn, proc_spec (readdir_spec pn) (readdir pn) recover abstr.
-  Axiom recover_noop : rec_noop recover abstr no_crash.
-  Axiom find_available_name_ok :
-    forall tid dirpn,
-    proc_spec (find_available_name_spec tid dirpn) (find_available_name dirpn) recover abstr.
-  Axiom debug_ok :  forall s, proc_spec (debug_spec) (debug s) recover abstr.
+Inductive fsOpT : Type -> Type :=
+| Create (dir : pathname) (name : string) : fsOpT nat
+| Mkdir (dir : pathname) (name : string) : fsOpT nat
+| Delete (pn : pathname) : fsOpT unit
+| Rmdir (pn : pathname) : fsOpT unit
+| Stat (dir : pathname) (name : string) : fsOpT stat_result
+| Readdir (pn : pathname) : fsOpT (list string)
+| Rename (src : pathname) (dstdir : pathname) (dstname : string) : fsOpT unit
+| Read (pn : pathname) : fsOpT string
+| Write (pn : pathname) (data : string) : fsOpT unit
+| FindAvailableName (dir : pathname) : fsOpT string
+| Debug (s : string) : fsOpT unit.
 
 
-  Hint Resolve init_ok.
-  Hint Resolve create_ok.
-  Hint Resolve mkdir_ok.
-  Hint Resolve delete_ok.
-  Hint Resolve rmdir_ok.
-  Hint Resolve rename_file_ok.
-  Hint Resolve read_ok.
-  Hint Resolve write_logged_ok.
-  Hint Resolve write_bypass_ok.
-  Hint Resolve stat_ok.
-  Hint Resolve readdir_ok.
-  Hint Resolve recover_noop.
-  Hint Resolve find_available_name_ok.
-  Hint Resolve debug_ok.
+Definition frame_pre_post (s s' : State) (p p' : pred _ _) : Prop :=
+  (exists F, s |= F * p) /\
+  (forall F, s |= F * p <-> s' |= F * p').
 
-End FSAPI.
+Arguments frame_pre_post s s' (p p')%pred.
+
+Parameter tid_to_string : nat -> string.
+
+Definition starts_with_tid tid (name : string) : Prop :=
+  exists namesuffix,
+    name = (tid_to_string tid ++ "." ++ namesuffix)%string.
+
+
+Inductive fs_step : forall T, fsOpT T -> nat -> State -> T -> State -> Prop :=
+| StepCreate : forall dir name tid s h s' dirnum,
+  frame_pre_post s s'
+    (dir |-> Dir dirnum * (dir ++ [name]) |-> Missing)
+    (dir |-> Dir dirnum * (dir ++ [name]) |-> File h empty_file) ->
+  fs_step (Create dir name) tid s h s'
+
+| StepMkdir : forall dir name tid s h s' dirnum newdirnum,
+  frame_pre_post s s'
+    (dir |-> Dir dirnum * (dir ++ [name]) |-> Missing)
+    (dir |-> Dir dirnum * (dir ++ [name]) |-> Dir newdirnum
+                        * subtree_pred (dir ++ [name]) empty_dir) ->
+  fs_step (Mkdir dir name) tid s h s'
+
+| StepDelete : forall pn h f tid s s',
+  frame_pre_post s s'
+    (pn |-> File h f)
+    (pn |-> Missing) ->
+  fs_step (Delete pn) tid s tt s'
+
+| StepRmdir : forall pn dirnum tid s s',
+  frame_pre_post s s'
+    (pn |-> Dir dirnum * subtree_pred pn empty_dir)
+    (pn |-> Missing) ->
+  fs_step (Rmdir pn) tid s tt s'
+
+| StepStat : forall dir name tid s r F dirnum,
+  s  |= F * dir |-> Dir dirnum ->
+  (r = StatFile ->
+    exists F' h f, F' * (dir ++ [name]) |-> File h f ===> F) ->
+  (r = StatDir ->
+    exists F' dirnum', F' * (dir ++ [name]) |-> Dir dirnum' ===> F) ->
+  (r = StatMissing ->
+    exists F', F' * (dir ++ [name]) |-> Missing ===> F) ->
+  fs_step (Stat dir name) tid s r s
+
+| StepReaddir : forall dir tid s r F dirnum,
+  s  |= F * dir |-> Dir dirnum ->
+  (forall fn,
+    (In fn r /\ exists F' handle f,
+     F' * (dir ++ [fn]) |-> File handle f ===> F) \/
+    (In fn r /\ exists F' dirinum,
+     F' * (dir ++ [fn]) |-> Dir dirinum ===> F) \/
+    (~ In fn r /\ exists F',
+     F' * (dir ++ [fn]) |-> Missing ===> F)) ->
+  fs_step (Readdir dir) tid s r s
+
+| StepRename : forall src dstdir dstname tid s handle f s' dirnum,
+  frame_pre_post s s'
+    (src |-> File handle f
+          * dstdir |-> Dir dirnum
+          * (dstdir ++ [dstname]) |-> Missing)
+    (src |-> Missing
+          * dstdir |-> Dir dirnum
+          * (dstdir ++ [dstname]) |-> File handle f) ->
+  fs_step (Rename src dstdir dstname) tid s tt s'
+
+| StepRead : forall pn tid s r handle F,
+  s  |= F * pn |-> File handle r ->
+  fs_step (Read pn) tid s (FileData r) s
+
+| StepWrite : forall pn tid s s' handle f0 data,
+  frame_pre_post s s'
+    (pn |-> File handle f0)
+    (pn |-> File handle (mk_file data)) ->
+  fs_step (Write pn data) tid s tt s'
+
+| StepFindAvailableName : forall dir dirnum tid s name F,
+  starts_with_tid tid name ->
+  s  |= F * dir |-> Dir dirnum * (dir ++ [name]) |-> Missing ->
+  fs_step (FindAvailableName dir) tid s name s
+
+| StepDebug : forall msg tid s,
+  fs_step (Debug msg) tid s tt s
+.
+
+
+Inductive mailfs_step_allowed : forall T, fsOpT T -> nat -> Prop :=
+| MailStepCreateTmp : forall dir name tid,
+  dir = tmpdir ->
+  starts_with_tid tid name ->
+  mailfs_step_allowed (Create dir name) tid
+
+| MailStepFindAvailableNameTmp : forall tid,
+  mailfs_step_allowed (FindAvailableName tmpdir) tid
+
+| MailStepFindAvailableNameUser : forall user dir tid,
+  dir = maildir ++ [user] ->
+  mailfs_step_allowed (FindAvailableName dir) tid
+
+| MailStepWriteTmp : forall pn dir name tid data,
+  dir = tmpdir ->
+  starts_with_tid tid name ->
+  pn = dir ++ [name] ->
+  mailfs_step_allowed (Write pn data) tid
+
+| MailStepRenameTmpToMailbox : forall src srcname dstdir user dstname tid,
+  src = tmpdir ++ [srcname] ->
+  starts_with_tid tid srcname ->
+  dstdir = maildir ++ [user] ->
+  starts_with_tid tid dstname ->
+  mailfs_step_allowed (Rename src dstdir dstname) tid
+.
+
+Definition mailfs_step T (op : fsOpT T) tid s r s' :=
+  fs_step op tid s r s' /\
+  mailfs_step_allowed op tid.
+
+
+
+Definition message := string.
+
+Inductive mailT : Type -> Type :=
+| Deliver (user : string) (m : message) : mailT unit.
+
+
+Definition deliver_core (user : string) (m : message) : proc fsOpT mailT unit :=
+  tmpname <- Op (FindAvailableName tmpdir);
+  _ <- Op (Create tmpdir tmpname);
+  _ <- Op (Write (tmpdir ++ [tmpname]) m);
+  fn <- Op (FindAvailableName (maildir ++ [user]));
+  _ <- Op (Rename (tmpdir ++ [tmpname]) (maildir ++ [user]) fn);
+  Ret tt.
+
+
+Ltac step_inv :=
+  match goal with
+  | H : fs_step _ _ _ _ _ |- _ =>
+    inversion H; clear H; subst; repeat sigT_eq
+  | H : mailfs_step _ _ _ _ _ |- _ =>
+    inversion H; clear H; subst; repeat sigT_eq
+  | H : mailfs_step_allowed _ _ |- _ =>
+    inversion H; clear H; subst; repeat sigT_eq
+  end.
+
+Ltac frame_inv :=
+  match goal with
+  | H : frame_pre_post _ _ _ _ |- _ =>
+    destruct H; repeat deex
+  end.
+
+Hint Constructors fs_step.
+Hint Constructors mailfs_step_allowed.
+
+Axiom tmpdir_not_maildir : forall user, tmpdir = maildir ++ [user] -> False.
+Hint Resolve tmpdir_not_maildir.
+
+
+Theorem find_available_name_tmpdir_both_mover :
+  both_mover mailfs_step (FindAvailableName tmpdir).
+Proof.
+  split; intros.
+  - unfold right_mover; intros.
+    exists s1.
+    repeat step_inv; unfold mailfs_step; intuition eauto.
+    all: try solve [ exfalso; eauto ].
+    all: frame_inv.
+    all: econstructor; eauto.
+    + eapply pimpl_trans. reflexivity.
+      2: eapply H2.
+      instantiate (3 := (_ * (tmpdir ++ [v0]) |-> Missing)%pred).
+      instantiate (2 := (_ * (tmpdir ++ [name]) |-> File v1 empty_file)%pred).
+      norm. cancel. reflexivity.
+
+      eapply pimpl_trans. reflexivity.
+      2: eapply pred_extract_merge.
+      2: eassumption.
+      2: apply H0.
+
+      repeat rewrite pred_eexcept_star.
+      repeat rewrite pred_eexcept_ptsto_ne.
+      norm. cancel. reflexivity.
+
+      admit.
+      admit.
+
+    + eapply pimpl_trans. reflexivity.
+      2: eapply H2.
+      admit.
+      admit.
+
+    + admit.
+
+  - admit.
+Admitted.
+
+Theorem create_tmpdir_both_mover : forall dir name,
+  both_mover mailfs_step (Create dir name).
+Proof.
+  split; intros.
+  - unfold right_mover; intros.
+    repeat step_inv; unfold mailfs_step; intuition eauto.
+
+    + exists (upd s (tmpdir ++ [name0]) (File v1 empty_file)).
+      repeat frame_inv.
+
+      eapply H2 in H0 as H0'.
+      eapply pred_extract_merge with (a := tmpdir ++ [name]) in H3 as H3'.
+      2: eapply pimpl_trans. 2: reflexivity. 3: eapply H0'.
+      2: norm. 2: cancel. 2: unfold stars; simpl. 2: reflexivity.
+
+      assert (Dir dirnum = Dir dirnum0).
+      eapply pred_merge_eq with (a := tmpdir).
+      eapply pimpl_trans. reflexivity. 2: eapply H3.
+      norm. cancel. unfold stars; simpl. reflexivity.
+      eapply pimpl_trans. reflexivity. 2: eapply H0'.
+      norm. cancel. unfold stars; simpl. reflexivity.
+      inversion H7; clear H7; subst.
+
+      eapply pred_extract_merge with (a := tmpdir ++ [name0]) in H0 as H0''.
+      2: eapply pimpl_trans. 2: reflexivity. 3: eapply H2.
+      3: eapply pimpl_trans. 3: reflexivity. 4: eapply H3'.
+      3: repeat rewrite pred_eexcept_star.
+      3: repeat rewrite pred_eexcept_ptsto_ne.
+      3: norm. 3: cancel. 3: unfold stars; simpl; reflexivity.
+      2: norm. 2: cancel. 2: unfold stars; simpl; reflexivity.
+
+Admitted.
