src/POCS.v
@@ -25,24 +25,9 @@ variety of proof automation (Ltac) used to simplify writing proofs with the POCS
 infrastructure. *)
 
 Require Export Helpers.Helpers.
+Require Export Helpers.ListStuff.
 
-(** [Helpers.Disk] defines our disk model. Disks are defined as lists of blocks,
-with many helper functions and theorems. *)
-
-Require Export Helpers.Disk.
-
-(** [Spec.Proc] defines [proc], the type of the programs you'll write in 6.826.
-We also describe how these programs run, including how programs can crash and
-how the system can run a recovery procedure afterward. *)
-
-Require Export Spec.Proc.
-
-(** [Spec.Abstraction] defines how we write specifications in terms of
-abstraction relations. *)
-
+Require Export Spec.ConcurProc.
+Require Export Spec.Equiv.
+Require Export Spec.Compile.
 Require Export Spec.Abstraction.
-
-(** [Spec.Recovery] proves a number of theorems for reasoning about recovery
-across abstraction layers. *)
-
-Require Export Spec.Recovery.
