Makefile
@@ -1,6 +1,11 @@
 ## Common library code
 CODE += $(wildcard src/Helpers/*.v)
 CODE += $(wildcard src/Spec/*.v)
+CODE += $(wildcard src/*.v)
+CODE += $(wildcard src/FS/SepLogic/Mem/*.v)
+CODE += $(wildcard src/FS/SepLogic/Pred/*.v)
+CODE += $(wildcard src/FS/SepLogic/*.v)
+CODE += $(wildcard src/FS/*.v)
 
 COQRFLAGS := -R build POCS
 
